{-# OPTIONS --exact-split --safe #-}
module Relation.Binary.ReflexiveTransitiveClosure.Property where

open import Relation.Binary.ReflexiveTransitiveClosure.Definition
  renaming (refl-trans-close to rtc)
open import Relation.Binary.Definition
open import Relation.Binary.Property

open import Universes
open import Function.Proof

private variable R : BinRel ğ’° X

instance
  Reflexive-rtc : Reflexive (rtc R)
  Transitive-rtc : Transitive (rtc R)
  InheritsSymmetric-rtc :
    â¦ƒ s : Symmetric R â¦„
    â†’ -----------------------------
    Symmetric (rtc R)
  Subrelation-rtc : R âŠ† rtc R
  Subrelation-rtc2 :
    rtc (rtc R) âŠ† rtc R
  Subrelation-2-Subrelation-rtc :
    {P : BinRel ğ’± X}
    â¦ƒ RâŠ†P : R âŠ† P â¦„
    â†’ ----------------------------------------
    rtc R âŠ† rtc P
  Relating-rtc :
    {P : BinRel ğ’° X}
    {R : BinRel ğ’± Y}
    {f : (x : X) â†’ Y}
    â¦ƒ _ : Relating f P R â¦„
    â†’ ----------------------
    Relating f (rtc P) (rtc R)

refl â¦ƒ Reflexive-rtc â¦„ = rfl
trans â¦ƒ Transitive-rtc â¦„ (rfl _) q = q
trans â¦ƒ Transitive-rtc â¦„ (step s p) q = step s (trans p q)
sym â¦ƒ InheritsSymmetric-rtc â¦„ (rfl a) = rfl a
sym â¦ƒ InheritsSymmetric-rtc â¦„ (step aRb p) = step-right (sym p) (sym aRb)

subrelâŠ† Subrelation-rtc {x} {y} xRy = step xRy (refl y)

subrelâŠ† Subrelation-rtc2 (rfl a) = refl a
subrelâŠ† Subrelation-rtc2 (step xR*z zR**y) =
  trans xR*z (subrel â¦ƒ Subrelation-rtc2 â¦„ zR**y)

subrelâŠ† Subrelation-2-Subrelation-rtc {x} {x} (rfl x) = refl x
subrelâŠ† Subrelation-2-Subrelation-rtc {x} {y} (step aRb bR*y) =
  step (subrel aRb) (subrel bR*y)

rel-preserv â¦ƒ Relating-rtc {f = f} â¦„ (rfl a) = rfl (f a)
rel-preserv â¦ƒ Relating-rtc â¦„ (step aRb aR*b) =
  step (rel-preserv aRb) (rel-preserv aR*b)

subrel-rtc-to-rtc-subrel-rtc :
  {P : BinRel ğ’± X}
  â¦ƒ s : P âŠ† rtc R â¦„
  â†’ -----------------------------------------
  rtc P âŠ† rtc R
subrel-rtc-to-rtc-subrel-rtc {R = _R_} {P = _P_} = go
  where go : rtc _P_ âŠ† rtc _R_
        subrelâŠ† go (rfl a) = refl a
        subrelâŠ† go (step {x} {b} {y} xPb bP*y) =
          trans (subrel xPb) (subrel â¦ƒ go â¦„ bP*y)
