{-# OPTIONS --exact-split --prop --safe #-}
module Relation.Binary.Pointwise.Property where

open import Relation.Binary.Pointwise.Definition
open import Relation.Binary
open import Relation.Binary.ReflexiveTransitiveClosure
  renaming (refl-trans-close to rtc)

open import Universes

instance
  PointwiseâŠ†Pointwise :
    {X : ğ’° Ë™}{A : X â†’ ğ’± Ë™}{B : X â†’ ğ’² Ë™}
    {R : âˆ€{x x'} â†’ Rel ğ’³ (A x) (B x')}
    {P : âˆ€{x x'} â†’ Rel ğ’¯ (A x) (B x')}
    â¦ƒ p : âˆ€ {x}{x'} â†’ R {x}{x'} âŠ† P {x}{x'} â¦„
    â†’ -----------------------------------
    Pointwise {X = X} (Î» {x}{x'} â†’ R {x}{x'}) âŠ† Pointwise P

subrelâŠ† PointwiseâŠ†Pointwise xRy x = subrel (xRy x)

{-
open import Type.Finite
open import Proposition.Sum
open import Proposition.Decidable
open import Data.Nat
open import Data.List hiding (last)
open import Data.Vec
open import Collection hiding (_~_)
open import Logic
open import Proof

open import Axiom.FunctionExtensionality

ptwise-rtc-commute :
  {R : BinRel ğ’° Y}
  â¦ƒ reflexive : Reflexive R â¦„
  (p : is-finite X)
  â¦ƒ dec : HasDecidableIdentity X â¦„
  â†’ ------------------------------------------
  Pointwise {X = X} (rtc R) ~ rtc (Pointwise R)
subrel â¦ƒ ~-âŠ† â¦ƒ ptwise-rtc-commute {Y = Y}{X = X}{R = R} (l , p) â¦„ â¦„ {f} {g} xâ†’f~g = {!!}
  where open import Proposition.Wrapped
        vec-to-f : (v : Vec Y (len l)) â†’ Wrapped (X â†’ Y)
        go :
          {f g : X â†’ Y}
          (l : List (Î£â‚š Î» x â†’
                     âˆƒ Î» yâ‚€ â†’ 
                     âˆƒ Î» yâ‚ â†’
                       yâ‚€ == f x âˆ§ yâ‚ == g x âˆ§ rtc R yâ‚€ yâ‚))
          (p : contains-all X (map elem l))
          â†’ --------------------
          âˆƒ Î» n â†’ âˆƒ Î» (l : Vec (Vec Y (len l)) (n +1)) â†’ {!vec-to-f!}
        go = {!!}
        vec-to-f v = wrap Î» x â†’ v ! index (p x) [ indexâ‰¤ (p x) ]
--   step (Î» x â†’ âŠ¥-recursion _ $ x âˆ‰âˆ… $ p x) (rfl g)
-- subrel â¦ƒ ~-âŠ† â¦ƒ ptwise-rtc-commute (x âˆ· l , p) â¦„ â¦„ {f} {g} xâ†’f~g = {!!}
subrel â¦ƒ ~-âŠ‡ â¦ƒ ptwise-rtc-commute p â¦„ â¦„ (rfl f) x = rfl (f x)
subrel â¦ƒ ~-âŠ‡ â¦ƒ ptwise-rtc-commute p â¦„ â¦„ (step f~g g~*h) x =
  step (f~g x) $ subrel â¦ƒ ~-âŠ‡ â¦ƒ ptwise-rtc-commute p â¦„ â¦„ g~*h x
-}
