{-# OPTIONS --exact-split --safe --prop #-}
module Proposition.Identity.Function where

open import Proposition.Identity.Definition

open import PropUniverses
open import Function.Property

type== : {x : X} {y : Y}
  (p : x Het.== y)
  â†’ ----------
  X == Y
type== {X = X}(Het.refl _) = Idâ‚š.refl X

subst :
  (ğ´ : (x : X) â†’ ğ’° áµ–)
  {x y : X}
  (p : x == y)
  (ax : ğ´ x)
  â†’ ----------
  ğ´ y
subst ğ´ (refl x) ax = ax

coe :
  (p : ğ‘‹ == ğ‘Œ)
  (x : ğ‘‹)
  â†’ ----------
  ğ‘Œ
coe (refl ğ‘‹) x = x

coe-eval :
  {ğ‘‹ : ğ’° áµ–}
  (p : ğ‘‹ == ğ‘Œ)
  (x : ğ‘‹)
  {A : {ğ‘‹ : ğ’° áµ–}(x : ğ‘‹) â†’ ğ’± Ë™}
  (f : {ğ‘‹ : ğ’° áµ–}(x : ğ‘‹) â†’ A x)
  â†’ ---------------
  f (coe p x) Het.== f x
coe-eval (refl _) x f = Het.refl (f x)

-- more general than Function.Proof.ap
-- it doesn't require the two sides
-- to be of the same type
ap : {I : ğ’° Ë™}{F : I â†’ ğ’± Ë™}{A : (i : I)(x : F i) â†’ ğ’² Ë™}
  (inject : Injective F)
  (f : âˆ€ {i}(x : F i) â†’ A i x)
  {i j : I}{x : F i}{y : F j}
  (p : x Het.== y)
  â†’ ----------
  f x Het.== f y
ap inject f p with inj (==â†’het== (type== p))
  where instance _ = inject
ap inject f (Het.refl x) | refl i = Het.refl (f x)

ap2 :
  {K : (x : X)(y : A x) â†’ ğ’° Ë™}
  (f : (x : X)(y : A x) â†’ K x y)
  {x x' : X}
  (p : x == x')
  {y : A x}{y' : A x'}
  (q : y Het.== y')
  â†’ ------------------------------
  f x y Het.== f x' y'
ap2 f (refl x) (Het.refl y) = Het.refl (f x y)

het-ap2 :
  {K : (x : X)(y : A x) â†’ ğ’° Ë™}
  (f : (x : X)(y : A x) â†’ K x y)
  {x x' : X}
  (p : x Het.== x')
  {y : A x}{y' : A x'}
  (q : y Het.== y')
  â†’ ------------------------------
  f x y Het.== f x' y'
het-ap2 f (Het.refl x)(Het.refl y) = Het.refl (f x y)

het-ap3 :
  {K : (x : X)(y : A x) â†’ ğ’° Ë™}
  {M : (x : X)(y : A x)(z : K x y) â†’ ğ’± Ë™}
  (f : (x : X)(y : A x)(z : K x y) â†’ M x y z)
  {x x' : X}
  (p : x == x')
  {y : A x}{y' : A x'}
  (q : y Het.== y')
  {z : K x y}{z' : K x' y'}
  (r : z Het.== z')
  â†’ ------------------------------
  f x y z Het.== f x' y' z'
het-ap3 f (refl x)(Het.refl y)(Het.refl z) = Het.refl (f x y z)
